NuBasicAbstractors.thy
@@ -38,28 +38,28 @@ lemma stepin: "\<^bold>p\<^bold>r\<^bold>o\<^bold>c f \<blangle> u \<tycolon> U 
 
 definition stepinR :: "( ('a::lrep) \<times>('z::lrep) \<Rightarrow> ('z1::lrep) state) \<Rightarrow> ((('c::lrep) \<times> 'a) \<times>'z \<Rightarrow> ('c \<times> 'z1) state)"
   where "stepinR f x = (case x of ((c,a),z) \<Rightarrow> bind (f (a,z)) (\<lambda>y. StatOn (c,y)))"
-lemma stepinR: "\<^bold>p\<^bold>r\<^bold>o\<^bold>c f \<blangle> (a \<tycolon> A)\<boxbar>Z \<longmapsto> Z1 \<brangle> \<Longrightarrow> \<^bold>p\<^bold>r\<^bold>o\<^bold>c stepinR f \<blangle> (c,a) \<tycolon> (C \<nuFusion> A)\<boxbar>Z \<longmapsto> c \<tycolon> C\<boxbar>Z1 \<brangle>"
+lemma stepinR: "\<^bold>p\<^bold>r\<^bold>o\<^bold>c f \<blangle> (a \<tycolon> A)\<heavy_comma>Z \<longmapsto> Z1 \<brangle> \<Longrightarrow> \<^bold>p\<^bold>r\<^bold>o\<^bold>c stepinR f \<blangle> (c,a) \<tycolon> (C \<nuFusion> A)\<heavy_comma>Z \<longmapsto> c \<tycolon> C\<heavy_comma>Z1 \<brangle>"
   unfolding stepinR_def \<nu>def bind_def by (auto 4 3)
 definition op_pairring_make :: "( ('z1::lrep) \<Rightarrow> ( ('b::lrep) \<times> ('z2::lrep) ) state) \<Rightarrow> ('a \<times> ('z1::lrep) \<Rightarrow> (( ('a::lrep) \<times> 'b) \<times> 'z2) state)"
   where "op_pairring_make f s = (case s of (a,z1) \<Rightarrow> bind (f z1) (\<lambda>(b,z2). StatOn ((a,b),z2)))"
-lemma op_pairring_make: "\<^bold>p\<^bold>r\<^bold>o\<^bold>c f \<blangle> Z1 \<longmapsto> b \<tycolon> B\<boxbar>Z2 \<brangle> \<Longrightarrow> \<^bold>p\<^bold>r\<^bold>o\<^bold>c op_pairring_make f \<blangle> a \<tycolon> A\<boxbar>Z1 \<longmapsto> (a,b) \<tycolon> A \<nuFusion> B\<boxbar>Z2 \<brangle>"
+lemma op_pairring_make: "\<^bold>p\<^bold>r\<^bold>o\<^bold>c f \<blangle> Z1 \<longmapsto> b \<tycolon> B\<heavy_comma>Z2 \<brangle> \<Longrightarrow> \<^bold>p\<^bold>r\<^bold>o\<^bold>c op_pairring_make f \<blangle> a \<tycolon> A\<heavy_comma>Z1 \<longmapsto> (a,b) \<tycolon> A \<nuFusion> B\<heavy_comma>Z2 \<brangle>"
   unfolding op_pairring_make_def \<nu>def bind_def by (auto 4 3)
 
 lemma [\<nu>auto_destruct]:
-  "\<^bold>p\<^bold>r\<^bold>o\<^bold>c g \<blangle> r \<tycolon> R\<boxbar>Z \<longmapsto> Z1 \<brangle> \<Longrightarrow>  \<^bold>p\<^bold>r\<^bold>o\<^bold>c f \<blangle> l \<tycolon> L\<boxbar>Z1 \<longmapsto> Z2 \<brangle> \<Longrightarrow> \<^bold>p\<^bold>r\<^bold>o\<^bold>c (stepinR g \<nuInstrComp> f) \<blangle> (l,r) \<tycolon> (L \<nuFusion> R)\<boxbar>Z \<longmapsto> Z2\<brangle>"
+  "\<^bold>p\<^bold>r\<^bold>o\<^bold>c g \<blangle> r \<tycolon> R\<heavy_comma>Z \<longmapsto> Z1 \<brangle> \<Longrightarrow>  \<^bold>p\<^bold>r\<^bold>o\<^bold>c f \<blangle> l \<tycolon> L\<heavy_comma>Z1 \<longmapsto> Z2 \<brangle> \<Longrightarrow> \<^bold>p\<^bold>r\<^bold>o\<^bold>c (stepinR g \<nuInstrComp> f) \<blangle> (l,r) \<tycolon> (L \<nuFusion> R)\<heavy_comma>Z \<longmapsto> Z2\<brangle>"
   unfolding AutoTag_def by (blast intro: instr_comp stepinR)
 lemma [\<nu>auto_construct]:
-  "\<^bold>p\<^bold>r\<^bold>o\<^bold>c f \<blangle> EoC Z \<longmapsto> l \<tycolon> L\<boxbar>EoC Z1 \<brangle> \<Longrightarrow>  \<^bold>p\<^bold>r\<^bold>o\<^bold>c g \<blangle>EoC Z1 \<longmapsto> r \<tycolon> R\<boxbar>EoC Z' \<brangle> \<Longrightarrow> \<^bold>p\<^bold>r\<^bold>o\<^bold>c (f \<nuInstrComp> op_pairring_make g) \<blangle>EoC Z \<longmapsto> (l,r) \<tycolon> (L \<nuFusion> R)\<boxbar>EoC Z'\<brangle>"
+  "\<^bold>p\<^bold>r\<^bold>o\<^bold>c f \<blangle> EoC Z \<longmapsto> l \<tycolon> L\<heavy_comma>EoC Z1 \<brangle> \<Longrightarrow>  \<^bold>p\<^bold>r\<^bold>o\<^bold>c g \<blangle>EoC Z1 \<longmapsto> r \<tycolon> R\<heavy_comma>EoC Z' \<brangle> \<Longrightarrow> \<^bold>p\<^bold>r\<^bold>o\<^bold>c (f \<nuInstrComp> op_pairring_make g) \<blangle>EoC Z \<longmapsto> (l,r) \<tycolon> (L \<nuFusion> R)\<heavy_comma>EoC Z'\<brangle>"
   unfolding AutoTag_def by (blast intro: instr_comp op_pairring_make)
 
-schematic_goal "\<^bold>p\<^bold>r\<^bold>o\<^bold>c ?f \<blangle> ?x \<tycolon> ((\<^bold>a\<^bold>t\<^bold>o\<^bold>m\<^bold>i\<^bold>c A \<nuFusion> \<^bold>a\<^bold>t\<^bold>o\<^bold>m\<^bold>i\<^bold>c B) \<nuFusion> \<^bold>a\<^bold>t\<^bold>o\<^bold>m\<^bold>i\<^bold>c D) \<nuFusion> \<^bold>a\<^bold>t\<^bold>o\<^bold>m\<^bold>i\<^bold>c C\<boxbar>Z \<longmapsto> (?Z1::(?'a::lrep) set) \<brangle>" by (rule \<nu>auto_destruct)+
+schematic_goal "\<^bold>p\<^bold>r\<^bold>o\<^bold>c ?f \<blangle> ?x \<tycolon> ((\<^bold>a\<^bold>t\<^bold>o\<^bold>m\<^bold>i\<^bold>c A \<nuFusion> \<^bold>a\<^bold>t\<^bold>o\<^bold>m\<^bold>i\<^bold>c B) \<nuFusion> \<^bold>a\<^bold>t\<^bold>o\<^bold>m\<^bold>i\<^bold>c D) \<nuFusion> \<^bold>a\<^bold>t\<^bold>o\<^bold>m\<^bold>i\<^bold>c C\<heavy_comma>Z \<longmapsto> (?Z1::(?'a::lrep) set) \<brangle>" by (rule \<nu>auto_destruct)+
 thm \<nu>auto_construct
 
 ML \<open>@{term "29::32"}\<close>
 lemma [simplified]: "(10::3) = (0::3)"  by auto
   thm term_def
 
-schematic_goal [simplified]:"\<^bold>c\<^bold>a\<^bold>s\<^bold>t (A\<boxbar>B\<boxbar>(x \<tycolon> C \<nuRefine> P)\<boxbar>D) \<longmapsto> (A\<boxbar>B\<boxbar>x \<tycolon> C\<boxbar>D) \<^bold>m\<^bold>e\<^bold>a\<^bold>n\<^bold>w\<^bold>h\<^bold>i\<^bold>l\<^bold>e ?P" by (rule \<nu>cast)+
-schematic_goal "\<^bold>c\<^bold>a\<^bold>s\<^bold>t (A\<boxbar>B) \<longmapsto> (A\<boxbar>B) \<^bold>m\<^bold>e\<^bold>a\<^bold>n\<^bold>w\<^bold>h\<^bold>i\<^bold>l\<^bold>e ?P" by (rule \<nu>cast)
+schematic_goal [simplified]:"\<^bold>c\<^bold>a\<^bold>s\<^bold>t (A\<heavy_comma>B\<heavy_comma>(x \<tycolon> C \<nuRefine> P)\<heavy_comma>D) \<longmapsto> (A\<heavy_comma>B\<heavy_comma>x \<tycolon> C\<heavy_comma>D) \<^bold>m\<^bold>e\<^bold>a\<^bold>n\<^bold>w\<^bold>h\<^bold>i\<^bold>l\<^bold>e ?P" by (rule \<nu>cast)+
+schematic_goal "\<^bold>c\<^bold>a\<^bold>s\<^bold>t (A\<heavy_comma>B) \<longmapsto> (A\<heavy_comma>B) \<^bold>m\<^bold>e\<^bold>a\<^bold>n\<^bold>w\<^bold>h\<^bold>i\<^bold>l\<^bold>e ?P" by (rule \<nu>cast)
 
 end
